src/PlutusIR/Transform/Alpha.v
@@ -208,15 +208,16 @@ Proof.
         eauto using alpha__is_error.
       * assumption.
     + assumption.
+  - (* E_Builtin_Apply_Eta *)
+    inversion H_alpha; subst.
+    (* Prove that partially_applied respects alpha. *)
+    admit.
   - (* E_Builtin_Apply *)
     inversion H_alpha; subst.
     specialize (alpha__compute_defaultfun H_alpha H0) as [ r' [H_compute H_alpha_r]].
     exists r'.
     split.
-    + assert (H_eq : applied_args (Apply s t) = applied_args (Apply t1' t2'))
-        by eauto using alpha__applied_args.
-      rewrite H_eq.
-      eauto using alpha__fully_applied, eval.
+    + eauto using alpha__fully_applied, eval.
     + eauto.
   - (* E_Error_Apply1 *)
     inversion H_alpha; subst.
@@ -226,4 +227,4 @@ Proof.
     inversion H_alpha; subst.
     specialize (IHH_eval t2' H4) as [r' [H_eval_t' H_alpha_r']].
     inversion H_alpha_r'.
-Qed.
+Admitted.
